Output modern HOL4 syntax, fix up builds of HOL4 examples (#114)
* convert ottScript.sml to modern HOL4

* modernize ottLib and add Holmakefile with basic test

* output HOL4 Inductive syntax for trindemossen-1 and later

* output HOL4 Type abbrevation syntax for kananaskis-14 and later

* adjust HOL4 newlines to be similar to Coq output

* make HOL4 rule label names follow Coq naming conventions

* fix up hol-def and coq-def build of ocaml_light example

* simplify ocaml_light Makefile, fix some hol theories for trindemossen-1

* fix up test10st_metatheoryScript.sml for trindemossen-1

* fix up leroy-jfp96.ott to check in HOL4 trindemossen-1

* make ocaml_light basicScript.sml compile with trindemossen-1

* update documentation for trindemossen-1 related changes

hol/selftest.sml
@@ -1,0 +1,6 @@
+open HolKernel boolLib Parse bossLib ottLib;
+
+val _ = ottDefine "test_def" `
+   (test T = T)
+/\ (test F = T)
+`;
