hol/ottScript.sml
@@ -1,82 +1,127 @@
-open HolKernel boolLib Parse bossLib pairTheory optionTheory stringTheory;
+open HolKernel boolLib Parse bossLib;
+open pairTheory optionTheory stringTheory;
 
 val _ = new_theory "ott";
 
-val list_minus_def = Define
-`(list_minus [] ys = [])  /\
- (list_minus (x::xs) ys = (if ~(MEM x ys) then x::(list_minus xs ys) else list_minus xs ys))`;
+Definition list_minus_def:
+ (list_minus [] ys = [])
+ /\
+ (list_minus (x::xs) ys =
+   if ~MEM x ys then x::(list_minus xs ys) else list_minus xs ys)
+End
 
-val list_minus_thm = Q.store_thm ("list_minus_thm",
-`!l x. MEM x (list_minus l l') = (MEM x l /\ ~MEM x l')`,
-Induct THEN RW_TAC list_ss [list_minus_def] THEN METIS_TAC []);
+Theorem list_minus_thm:
+ !l x. MEM x (list_minus l l') <=> (MEM x l /\ ~MEM x l')
+Proof
+ Induct >> RW_TAC list_ss [list_minus_def] >> METIS_TAC []
+QED
 
-val list_minus_append = Q.store_thm ("list_minus_append",
-`!l1 l2 l3. list_minus (l1++l2) l3 = list_minus l1 l3 ++ list_minus l2 l3`,
-Induct THEN RW_TAC list_ss [list_minus_def]);
+Theorem list_minus_append:
+ !l1 l2 l3. list_minus (l1++l2) l3 = list_minus l1 l3 ++ list_minus l2 l3
+Proof
+ Induct >> RW_TAC list_ss [list_minus_def]
+QED
 
-val list_assoc_def = Define
-`(list_assoc x [] = NONE)  /\
- (list_assoc x ((x',y')::xys) = (if x=x' then SOME y' else list_assoc x xys))`;
+Definition list_assoc_def:
+ (list_assoc x [] = NONE)
+ /\
+ (list_assoc x ((x',y')::xys) = if x=x' then SOME y' else list_assoc x xys)
+End
 
-val list_assoc_mem = Q.store_thm ("list_assoc_mem",
-`!l x y. (list_assoc x l = SOME y) ==> MEM (x,y) l`,
-Induct THEN RW_TAC list_ss [list_assoc_def] THEN
-Cases_on `h` THEN RW_TAC list_ss [list_assoc_def] THEN
-Cases_on `x = q` THEN FULL_SIMP_TAC list_ss [list_assoc_def]);
+Theorem list_assoc_mem:
+ !l x y. list_assoc x l = SOME y ==> MEM (x,y) l
+Proof
+ Induct >> RW_TAC list_ss [list_assoc_def] >>
+ Cases_on `h` >> RW_TAC list_ss [list_assoc_def] >>
+ Cases_on `x = q` >> FULL_SIMP_TAC list_ss [list_assoc_def]
+QED
 
-val list_assoc_not_mem = Q.store_thm ("list_assoc_not_mem",
-`!l x y. (list_assoc x l = NONE) ==> ~MEM (x,y) l`,
-Induct THEN FULL_SIMP_TAC list_ss [list_assoc_def] THEN Cases_on `h` THEN RW_TAC list_ss [list_assoc_def]);
+Theorem list_assoc_not_mem:
+ !l x y. list_assoc x l = NONE ==> ~MEM (x,y) l
+Proof
+ Induct >> FULL_SIMP_TAC list_ss [list_assoc_def] >>
+ Cases_on `h` >> RW_TAC list_ss [list_assoc_def]
+QED
 
-val list_assoc_split = Q.store_thm ("list_assoc_split",
-`!l x y. (list_assoc x l = SOME y) = ?l1 l2. (l = l1++(x,y)::l2) /\ ~MEM x (MAP FST l1)`,
-Induct THEN RW_TAC list_ss [list_assoc_def] THEN Cases_on `h` THEN RW_TAC list_ss [list_assoc_def] THEN
-EQ_TAC THEN RW_TAC list_ss [] THENL
-[MAP_EVERY Q.EXISTS_TAC [`[]`, `l`] THEN RW_TAC list_ss [],
- Cases_on `l1` THEN FULL_SIMP_TAC list_ss [] THEN RW_TAC list_ss [] THEN FULL_SIMP_TAC list_ss [],
- MAP_EVERY Q.EXISTS_TAC [`(q,r)::l1`, `l2`] THEN RW_TAC list_ss [],
- Cases_on `l1` THEN FULL_SIMP_TAC list_ss [] THEN METIS_TAC []]);
+Theorem list_assoc_split:
+ !l x y. list_assoc x l = SOME y <=>
+  ?l1 l2. (l = l1++(x,y)::l2) /\ ~MEM x (MAP FST l1)
+Proof
+ Induct >> RW_TAC list_ss [list_assoc_def] >>
+ Cases_on `h` >> RW_TAC list_ss [list_assoc_def] >>
+ EQ_TAC >> RW_TAC list_ss [] >| [
+  MAP_EVERY Q.EXISTS_TAC [`[]`, `l`] >> RW_TAC list_ss [],
+  Cases_on `l1` >> FULL_SIMP_TAC list_ss [] >>
+  RW_TAC list_ss [] >> FULL_SIMP_TAC list_ss [],
+  MAP_EVERY Q.EXISTS_TAC [`(q,r)::l1`, `l2`] >> RW_TAC list_ss [],
+  Cases_on `l1` >> FULL_SIMP_TAC list_ss [] >> METIS_TAC []
+ ]
+QED
 
-val list_assoc_append = Q.store_thm ("list_assoc_append",
-`!l1 l2 x. list_assoc x (l1++l2) =
-              case list_assoc x l1 of
-                 SOME y => SOME y
-               | NONE => list_assoc x l2`,
-Induct THEN RW_TAC list_ss [list_assoc_def] THEN Cases_on `h` THEN RW_TAC list_ss [list_assoc_def]);
+Theorem list_assoc_append:
+ !l1 l2 x. list_assoc x (l1++l2) =
+   case list_assoc x l1 of
+   | SOME y => SOME y
+   | NONE => list_assoc x l2
+Proof
+ Induct >> RW_TAC list_ss [list_assoc_def] >>
+ Cases_on `h` >> RW_TAC list_ss [list_assoc_def]
+QED
 
-val mem_list_assoc = Q.store_thm ("mem_list_assoc",
-`!l x. MEM x (MAP FST l) ==> ?y. list_assoc x l = SOME y`,
-Induct THEN RW_TAC list_ss [list_assoc_def] THEN Cases_on `h` THEN RW_TAC list_ss [list_assoc_def]);
+Theorem mem_list_assoc:
+ !l x. MEM x (MAP FST l) ==> ?y. list_assoc x l = SOME y
+Proof
+ Induct >> RW_TAC list_ss [list_assoc_def] >>
+ Cases_on `h` >> RW_TAC list_ss [list_assoc_def]
+QED
 
-val not_mem_list_assoc = Q.store_thm ("not_mem_list_assoc",
-`!l x. ~MEM x (MAP FST l) ==> (list_assoc x l = NONE)`,
-Induct THEN RW_TAC list_ss [list_assoc_def] THEN Cases_on `h` THEN RW_TAC list_ss [list_assoc_def] THEN
-METIS_TAC [FST]);
+Theorem not_mem_list_assoc:
+ !l x. ~MEM x (MAP FST l) ==> list_assoc x l = NONE
+Proof
+ Induct >> RW_TAC list_ss [list_assoc_def] >>
+ Cases_on `h` >> RW_TAC list_ss [list_assoc_def] >>
+ METIS_TAC [FST]
+QED
 
-val list_assoc_distinct_reverse = Q.store_thm ("list_assoc_distinct_reverse",
-`!l. ALL_DISTINCT (MAP FST l) ==> !x. list_assoc x (REVERSE l) = list_assoc x l`,
-Induct THEN RW_TAC list_ss [list_assoc_def, list_assoc_append] THEN Cases_on `h` THEN
-RW_TAC list_ss [list_assoc_def] THEN FULL_SIMP_TAC list_ss [] THENL
-[METIS_TAC [not_mem_list_assoc, option_case_def],
- Cases_on `list_assoc x l` THEN RW_TAC list_ss []]);
+Theorem list_assoc_distinct_reverse:
+ !l. ALL_DISTINCT (MAP FST l) ==>
+  !x. list_assoc x (REVERSE l) = list_assoc x l
+Proof
+ Induct >> RW_TAC list_ss [list_assoc_def,list_assoc_append] >>
+ Cases_on `h` >> RW_TAC list_ss [list_assoc_def] >>
+ FULL_SIMP_TAC list_ss [] >| [
+  METIS_TAC [not_mem_list_assoc, option_case_def],
+  Cases_on `list_assoc x l` >> RW_TAC list_ss []
+ ]
+QED
 
-val list_assoc_map = Q.store_thm ("list_assoc_map",
-`!l x f. (list_assoc x (MAP (\z. (FST z, f (SND z))) l) = OPTION_MAP f (list_assoc x l))`,
-Induct THEN RW_TAC list_ss [list_assoc_def] THEN Cases_on `h` THEN RW_TAC list_ss [list_assoc_def] THEN
-METIS_TAC [FST]);
+Theorem list_assoc_map:
+ !l x f. list_assoc x (MAP (\z. (FST z, f (SND z))) l) =
+  OPTION_MAP f (list_assoc x l)
+Proof
+ Induct >> RW_TAC list_ss [list_assoc_def] >>
+ Cases_on `h` >> RW_TAC list_ss [list_assoc_def] >>
+ METIS_TAC [FST]
+QED
 
-val mono_every_id_thm = Q.store_thm ("mono_every_id_thm",
-`(!x. P x ==> Q x) ==> EVERY (\x. x) (MAP P l) ==> EVERY (\x. x) (MAP Q l)`,
-Induct_on `l` THEN RW_TAC list_ss [] THEN METIS_TAC []);
+Theorem mono_every_id_thm:
+ (!x. P x ==> Q x) ==> EVERY (\x. x) (MAP P l) ==> EVERY (\x. x) (MAP Q l)
+Proof
+ Induct_on `l` >> RW_TAC list_ss [] >> METIS_TAC []
+QED
 
 val _ = IndDefLib.export_mono "mono_every_id_thm";
 
-val filter_size = Q.store_thm ("filter_size",
-`!l f size. list_size size (FILTER f l) <= list_size size l`,
-Induct THEN RW_TAC list_ss [listTheory.list_size_def] THEN
-Q.PAT_ASSUM `!f' size. g f' size` (STRIP_ASSUME_TAC o (Q.SPECL [`f`, `size`])) THEN
-DECIDE_TAC);
+Theorem filter_size:
+ !l f size. list_size size (FILTER f l) <= list_size size l
+Proof
+ Induct >> RW_TAC list_ss [listTheory.list_size_def] >>
+ Q.PAT_ASSUM `!f' size. g f' size` (STRIP_ASSUME_TAC o (Q.SPECL [`f`, `size`])) >>
+ DECIDE_TAC
+QED
 
-val clause_name = Define `clause_name (x:string) = T`;
+Definition clause_name_def:
+ clause_name (x:string) = T
+End
 
-val _ = export_theory();
+val _ = export_theory ();
